Adding HKDF (partly verified)

providers/evercrypt/EverCrypt.Helpers.fsti
@@ -25,3 +25,4 @@ let uint32_p = B.buffer uint32_t
 let uint64_p = B.buffer uint64_t
 
 let uint8_pl (l:nat) = p:uint8_p {B.length p = l}
+let uint8_l (p:uint8_p) = l:UInt32.t {B.length p = UInt32.v l}
