providers/evercrypt/EverCrypt.HMAC.fsti
@@ -50,3 +50,5 @@ val compute:
     LowStar.Modifies.(modifies (loc_buffer tag) h0 h1) /\
     ( length data + blockLength (Ghost.hide a) <= maxLength (Ghost.hide a) /\ (* required for subtyping the RHS below *)    
       as_seq h1 tag == hmac (Ghost.hide a) (as_seq h0 key) (as_seq h0 data)))
+
+//18-07-13 pick uniform names? hash{spec} vs compute{hmac}
