providers/evercrypt/fst/EverCrypt.HKDF.fst
@@ -1,0 +1,148 @@
+module EverCrypt.HKDF
+
+/// 18-03-04 to be compared to Hashing.HKDF, salvaged as a spec 
+
+module ST = FStar.HyperStack.ST
+open FStar.HyperStack.All
+
+open FStar.Mul
+open FStar.HyperStack
+open FStar.HyperStack.ST
+open LowStar.Buffer
+open LowStar.BufferOps
+open FStar.Integers
+
+open EverCrypt.Hash 
+
+type alg = EverCrypt.HMAC.ha
+
+
+//18-03-05 I'd rather verify a simpler implementation, closer to the spec, as outlined below. 
+//18-03-05 We could make do with fewer loop variables if it helps with C.Loops
+private val hkdf_expand_loop: 
+  a       : alg -> (
+  okm     : uint8_p ->
+  prk     : uint8_p ->
+  prklen  : uint8_l prk ->
+  infolen : UInt32.t -> 
+  len     : uint8_l okm  ->
+  hashed  : uint8_pl (tagLength (Ghost.hide a) + v infolen + 1) ->
+  i       : UInt8.t {
+    let a = Ghost.hide a in 
+    let count = v i in 
+    let required = v len in 
+    HMAC.keysized a (length prk) /\ 
+    disjoint okm prk /\
+    disjoint hashed okm /\ 
+    disjoint hashed prk /\
+    tagLength a + v infolen + 1 + blockLength a < pow2 32 /\ (* specific to this implementation *)
+    tagLength a + pow2 32 + blockLength a <= maxLength a /\
+    count < 255 /\
+    required <= (255 - count) * tagLength a } ->
+  ST unit
+  (requires fun h0 -> 
+    live h0 okm /\ live h0 prk /\ live h0 hashed)
+  (ensures  fun h0 r h1 -> 
+    //live h1 okm /\ 
+    LowStar.Modifies.(modifies (loc_union (loc_buffer okm) (loc_buffer hashed)) h0 h1) /\ (
+    let prk = as_seq h0 prk in 
+    let info = as_seq h0 (gsub hashed (tagLen a) infolen) in 
+    let last = if i = 0uy then Seq.empty else as_seq h0 (gsub hashed 0ul (tagLen a)) in 
+    let okm = as_seq h1 okm in 
+    okm == expand0 (Ghost.hide a) prk info (v len) (v i) last)))
+
+#set-options "--z3rlimit 100"
+let rec hkdf_expand_loop a okm prk prklen infolen len hashed i =
+  push_frame ();
+  let tlen = tagLen a in 
+  let tag = sub hashed 0ul tlen in 
+  let info_counter = offset hashed tlen in 
+  let info = sub info_counter 0ul infolen in
+  let counter = offset info_counter infolen in 
+  assert(disjoint tag info /\ disjoint tag counter /\ disjoint info counter);
+
+  let i' = i + 1uy in
+
+  let h0 = ST.get() in  // initial state
+  counter.(0ul) <- i';
+
+  let h1 = ST.get() in // before hashing
+  FStar.Seq.(lemma_eq_intro (upd (as_seq h0 counter) 0 i') (create 1 i'));
+  assert(as_seq h1 counter == Seq.create 1 i');
+
+  // derive an extra tag 
+  if i = 0uy then (
+    // the first input is shorter, does not include the chaining block
+    let len1 = infolen + 1ul in 
+    HMAC.compute a tag prk prklen info_counter len1;
+
+    let h2 = ST.get() in 
+    ( let info1 = as_seq h1 info in 
+      let ctr1 = as_seq h1 counter in 
+      let prk1 = as_seq h1 prk in 
+      let tag2 = as_seq h2 tag in 
+      let text = Seq.empty @| info1 @| ctr1 in
+
+      // assert(tag2 == HMAC.hmac a v_prk (as_seq h1 hashed1)); 
+      Seq.lemma_eq_intro (as_seq h1 info_counter) text;
+      assert(tag2 == HMAC.hmac (Ghost.hide a) prk1 text)  ))
+  else (
+    HMAC.compute a tag prk prklen hashed (tlen + infolen + 1ul);
+    let h2 = ST.get() in 
+    ( let info1 = as_seq h1 info in 
+      let ctr1 = as_seq h1 counter in 
+      let prk1 = as_seq h1 prk in 
+      let tag1 = as_seq h1 tag in 
+      let tag2 = as_seq h2 tag in 
+      let text = tag1 @| info1 @| ctr1 in
+      assert(tag2 == HMAC.hmac (Ghost.hide a) prk1 (as_seq h1 hashed)); 
+      Seq.lemma_eq_intro (as_seq h1 hashed) text ; 
+      assert(tag2 == HMAC.hmac (Ghost.hide a) prk1 text )
+    ));
+
+  // copy it to the result, and iterate if required
+  if len <= tlen then 
+    blit tag 0ul okm 0ul len
+  else (
+    blit tag 0ul okm 0ul tlen;
+    let len = len - tlen in 
+    let okm = sub okm tlen len in 
+    let h2 = ST.get() in 
+    hkdf_expand_loop a okm prk prklen infolen len hashed i';
+
+    let h3 = ST.get() in 
+    assert(
+      let prk = as_seq h0 prk in 
+      let info = as_seq h0 (gsub hashed (tagLen a) infolen) in 
+      let last = if i' = 0uy then Seq.empty else as_seq h2 (gsub hashed 0ul (tagLen a)) in 
+      let okm = as_seq h3 okm in 
+      okm ==  expand0 (Ghost.hide a) prk info (v len) (v i') last)
+    );
+
+  // TODO complete functional correctness
+  let h3 = ST.get() in 
+  assume(
+      let prk = as_seq h0 prk in 
+      let info = as_seq h0 (gsub hashed (tagLen a) infolen) in 
+      let last = if i = 0uy then Seq.empty else as_seq h0 (gsub hashed 0ul (tagLen a)) in 
+      let okm = as_seq h3 okm in 
+      okm ==  expand0 (Ghost.hide a) prk info (v len) (v i) last);
+
+  pop_frame()
+
+// | tagLen a | infolen | 1 | 
+  
+let hkdf_extract a prk salt saltlen ikm ikmlen =
+    HMAC.compute a prk salt saltlen ikm ikmlen
+
+#set-options "--z3rlimit 20"
+let hkdf_expand a okm prk prklen info infolen len = 
+  push_frame();
+  let tlen = tagLen a in 
+  let text = alloca 0uy (tlen + infolen + 1ul) in 
+  blit info 0ul text tlen infolen; 
+  assert_norm(
+    let a = Ghost.hide a in 
+    tagLength a + pow2 32 + blockLength a <= maxLength a);
+  hkdf_expand_loop a okm prk prklen infolen len text 0uy;
+  pop_frame()
